fix: update Addition32.lean for SentenceOrder refactoring

Clean/Examples/AddOperations.lean
@@ -6,8 +6,8 @@ section
 def circuit := do
   let x ← witnessField (F := F pBabybear) fun _ => 246
   let y ← witnessField fun _ => 20
-  let z ← Gadgets.Addition8.circuit.main { x, y }
-  Gadgets.Addition8.circuit.main { x, y := z }
+  let z ← Gadgets.Addition8.circuit (emptyOrder (F pBabybear)) |>.main { x, y }
+  Gadgets.Addition8.circuit (emptyOrder (F pBabybear)) |>.main { x, y := z }
 
 -- #eval circuit.operations
 
